lib/corres_method: more robust schematics
corres method now fails outright if the subgoal
conclusion is schematic, otherwise it can loop.

Handle cases where corressimp
would leave preconditions uninstantiated if the
goal was solved by clarsimp.

lib/Corres_Method.thy
@@ -638,7 +638,14 @@ private method corres_apply =
 
 private method corres_alternate = corres_inst | corres_rv
 
+private definition "my_true \<equiv> True"
+
+private lemma my_true: "my_true" by (simp add: my_true_def)
+
+method no_schematic_concl = (fails \<open>rule my_true\<close>)
+
 method corres_once declares corres_splits corres corresK corresc_simp =
+  (no_schematic_concl,
    (corres_alternate |
      (corres_fold_dc?,
      (corres_pre,
@@ -648,7 +655,7 @@ method corres_once declares corres_splits corres corresK corresc_simp =
       | corres_concrete_r
       | corresc
       | (rule corres_splits, corres_once)
-      ))))
+      )))))
 
 
 method corres declares corres_splits corres corresK corresc_simp =
@@ -1007,13 +1014,34 @@ lemmas [correswp_wp_comb] =
 declare hoare_post_comb_imp_conj[correswp_wp_comb_del]
 
 section \<open>Corressimp\<close>
+text \<open>Combines corres, wp and clarsimp\<close>
 
-text \<open>Wrap all the previous methods up in one big hammer.\<close>
+text
+\<open>If clarsimp solves a terminal subgoal, its preconditions are left uninstantiated. We can
+try to catch this by first attempting a trivial instantiation before invoking clarsimp, but
+only keeping the result if clarsimp solves the goal,\<close>
+
+lemmas hoare_True_inst =
+  hoare_pre[where P="\<lambda>_. True", of "\<lambda>_. True", # \<open>-\<close> \<open>simp\<close>]
+  asm_rl[of "\<lbrace>\<lambda>_. True\<rbrace> f \<lbrace>E\<rbrace>,\<lbrace>R\<rbrace>" for f E R]
+
+lemmas corres_rv_True_inst =
+  asm_rl[of "corres_rv True r (\<lambda>_. True) (\<lambda>_. True) f f' Q" for r f f' Q]
+  asm_rl[of "corres_rvE_R True r (\<lambda>_. True) (\<lambda>_. True) f f' Q" for r f f' Q]
+
+lemmas corresK_True_inst =
+  asm_rl[of "corres_underlyingK sr nf nf' True dc (\<lambda>_. True) (\<lambda>_. True) f g" for sr nf nf' f g]
+  asm_rl[of "corres_underlyingK sr nf nf' True r (\<lambda>_. True) (\<lambda>_. True) f g" for sr nf nf' r f g]
+  asm_rl[of "corres_underlying sr nf nf' dc (\<lambda>_. True) (\<lambda>_. True) f g" for sr nf nf' f g]
+  asm_rl[of "corres_underlying sr nf nf' r (\<lambda>_. True) (\<lambda>_. True) f g" for sr nf nf' r f g]
+
+lemmas calculus_True_insts = hoare_True_inst corres_rv_True_inst corresK_True_inst
 
 method corressimp uses simp cong search wp
   declares corres corresK corres_splits corresc_simp =
   ((corres corresc_simp: simp
     | correswp wp: wp
+    | (rule calculus_True_insts, solves \<open>clarsimp cong: cong simp: simp corres_protect_def\<close>)
     | clarsimp cong: cong simp: simp simp del: corres_simp_del split del: if_split
     | (match search in _ \<Rightarrow> \<open>corres_search search: search\<close>))+)[1]
 
